src/ShouldBuild.v
@@ -16,9 +16,10 @@ From Perennial.program_proof Require
      util_proof
      lockmap_proof
      (* temporarily disabled while wal abstraction is in flux *)
-     (* wal.proof wal.heapspec txn.specs *)
+     (* wal.proof *)
      wal.specs
-     wal.circular_proof.
+     wal.circular_proof
+     txn.specs.
 From Perennial.goose_lang Require
      ffi.append_log_ffi.
 
