src/program_proof/wal/heapspec.v
@@ -459,6 +459,7 @@ Proof.
     {
       rewrite H6.
       (* use H1 at address k *)
+      admit.
     }
 Admitted.
 
